% small.tex
\documentclass{beamer}
%\usetheme{default}
\usetheme{Warsaw}

\usepackage{tikzsymbols}
\usepackage{tkz-berge, tkz-graph}
\usepackage{caption}
\usepackage{colortbl}

% Define some colors:

%\definecolor{DarkFern}{HTML}{407428}
%\definecolor{DarkCharcoal}{HTML}{4D4944}
%\colorlet{Fern}{DarkFern!85!white}
%\colorlet{Charcoal}{DarkCharcoal!85!white}
%\colorlet{LightCharcoal}{Charcoal!50!white}
%\colorlet{AlertColor}{orange!80!black}
%\colorlet{DarkRed}{red!70!black}
%\colorlet{DarkBlue}{blue!70!black}
%\colorlet{DarkGreen}{green!70!black}


% Use the colors:

%\setbeamercolor{title}{fg=Fern}
%\setbeamercolor{frametitle}{fg=Fern}
%\setbeamercolor{normal text}{fg=Charcoal}
%\setbeamercolor{block title}{fg=black,bg=Fern!25!white}
%\setbeamercolor{block body}{fg=black,bg=Fern!25!white}
%\setbeamercolor{alerted text}{fg=AlertColor}
%\setbeamercolor{itemize item}{fg=Charcoal}


\newcommand{\N}{\mathbb{N}}
\newcommand{\Z}{\mathbb{Z}}
\newcommand{\R}{\mathbb{R}}
\newcommand{\Q}{\mathbb{Q}}

\newcommand{\F}{\mathbb{F}}

\newcommand{\bd}{\textbf}
\newcommand{\on}{yellow}
\newcommand{\off}{white}
\usepackage{mathtools}
\DeclarePairedDelimiter\abs{\lvert}{\rvert}%
\DeclarePairedDelimiter\norm{\lVert}{\rVert}%

\begin{document}


\title[The Cyclic Lightbulb Game] % (optional, only for long titles)
{The Cyclic Lightbulb Game}
%\subtitle{Subtitle}
\author[Last Names] % (optional, for multiple authors)
{Names}
\institute[University of Pittsburgh] % (optional)
{
  \inst{}%
  University of Pittsburgh
}
\date[January 31, 2019] % (optional)
{Math 1800,

January 31, 2019}
\subject{Lightbulb Game}

\frame{\titlepage}

%%%%%%%%%%%%%%%%%%%%%%%%%%%%%%%%%%%%

\begin{frame}
\frametitle{The Lightbulb Game}

Suppose we have the lightbulbs\ldots

\begin{figure}[!h]
    \centering
    \begin{tikzpicture}
        %\GraphInit[vstyle=Classic]
        \SetVertexMath
        %\tikzset{VertexStyle/.style = {shape = circle,fill = black, minimum size = 5pt,inner sep=0pt}}
        %\SetVertexNoLabel
        \SetVertexLabelOut
        \SetVertexNormal[Shape=circle, FillColor=\off, LineWidth=1pt]
        \Vertex[Lpos=-90]{A}
        \SetVertexNormal[Shape=circle, FillColor=\on, LineWidth=1pt]
        \EA[Lpos=-90](A) {B}
        \SetVertexNormal[Shape=circle, FillColor=\off, LineWidth=1pt]
        \EA[Lpos=-90](B) {C}
        \Edges(A,B,C)
    \end{tikzpicture}
    %\captionsetup{labelformat=empty}
\end{figure}

Or more generally,
\begin{figure}[!h]
    \centering
    \begin{tikzpicture}
        %\GraphInit[vstyle=Classic]
        \SetVertexMath
        %\tikzset{VertexStyle/.style = {shape = circle,fill = black, minimum size = 5pt,inner sep=0pt}}
        %\SetVertexNoLabel
        \SetVertexLabelOut
        \SetVertexNormal[Shape=circle, FillColor=\off, LineWidth=1pt]
        \Vertex[Lpos=-90]{1}
        \SetVertexNormal[Shape=circle, FillColor=\on, LineWidth=1pt]
        \EA[Lpos=-90](1) {2}
        \SetVertexNormal[Shape=circle, FillColor=\off, LineWidth=1pt]
        \EA[Lpos=-90](2) {3}
        \SetGraphUnit{2}
        \EA[Lpos=-90](3) {n}
        \Edges(1,2,3)
        \Edge[label={...}](3)(n)
    \end{tikzpicture}
    %\captionsetup{labelformat=empty}
\end{figure}

\end{frame}

\begin{frame}
    \frametitle{The Cyclic Lightbulb Game}
    PLACEHOLDER
    Maybe something about how our data suggested some configs weren't solvable when
    $n\equiv 0 \pmod{3}$\ldots

\begin{figure}[!h]
    \centering
    \begin{tikzpicture}
        %\GraphInit[vstyle=Classic]
        \SetVertexMath
        %\tikzset{VertexStyle/.style = {shape = circle,fill = black, minimum size = 5pt,inner sep=0pt}}
        %\SetVertexNoLabel
        \SetVertexLabelOut
        \SetGraphUnit{2}
        \begin{scope}[rotate=0]
            \SetVertexNormal[Shape=circle, FillColor=\off, LineWidth=1pt]
            \Vertices{circle}{1,2,3,4,n}
            \Edges(1,2,3,4) \Edges(n,1)
            \Edge[label={...}](4)(n)
        \end{scope}
    \end{tikzpicture}
    %\captionsetup{labelformat=empty}
\end{figure}
\end{frame}

%%%%%%%%%%%%%%%%%%%%%%%%%%%%%%%%%%%%

\begin{frame}
\frametitle{The Recursive Formula}

We will show the adjacency matrix $A_n$ of the cyclic graph $C_n$, has its determinant
given by
\[
    \abs{A_n} = \abs{T_{n-1}} - 2\abs{T_{n-2}} + 2(-1)^{n+1}
\]
\end{frame}

\begin{frame}
\frametitle{The Recursive Formula}
    $A_n$ has the form:
    \[
        A_n=
        \begin{pmatrix}
            1 & 1 & 0 & 0 & \dots & 0 & 1\\
            1 & 1 & 1 & 0 & \dots & \dots & 0\\
            0 & 1 & \ddots & \ddots & \ddots & \ddots & \vdots\\
            0 & 0 & \ddots & \ddots & \ddots & \vdots & \vdots\\
            \vdots & \vdots & \ddots & \ddots & \ddots & \ddots & 0\\
            0 & \vdots & \dots & \ddots & \ddots & \ddots & 1\\
            1 & 0 & \dots & \dots & 0 & 1 & 1
        \end{pmatrix}
    \]
\end{frame}

\begin{frame}
\frametitle{The Recursive Formula}
    We preform cofactor expansion along the first row of $A_n$. This will yield 3 terms.
    \[
        A_n=
        \left(\begin{array}{ccccccc}
            \rowcolor{red!20}
            1 & 1 & 0 & 0 & \dots & 0 & 1\\
            1 & 1 & 1 & 0 & \dots & \dots & 0\\
            0 & 1 & \ddots & \ddots & \ddots & \ddots & \vdots\\
            0 & 0 & \ddots & \ddots & \ddots & \vdots & \vdots\\
            \vdots & \vdots & \ddots & \ddots & \ddots & \ddots & 0\\
            0 & \vdots & \dots & \ddots & \ddots & \ddots & 1\\
            1 & 0 & \dots & \dots & 0 & 1 & 1
        \end{array}\right)
    \]
\end{frame}

\begin{frame}
\frametitle{The Recursive Formula}

    \bigskip

    \textbf{First term}
    \small
    \[
        A_n=
        \left(\begin{array}{>{\columncolor{red!20}}ccccccc}
            \rowcolor{red!20}
            1 & 1 & 0 & 0 & \dots & 0 & 1\\
            1 & 1 & 1 & 0 & \dots & \dots & 0\\
            0 & 1 & \ddots & \ddots & \ddots & \ddots & \vdots\\
            0 & 0 & \ddots & \ddots & \ddots & \vdots & \vdots\\
            \vdots & \vdots & \ddots & \ddots & \ddots & \ddots & 0\\
            0 & \vdots & \dots & \ddots & \ddots & \ddots & 1\\
            1 & 0 & \dots & \dots & 0 & 1 & 1
        \end{array}\right)
        \hspace{.1in}
        (-1)^{1+1}
        \begin{vmatrix}
            1 & 1 & 0 & \dots & 0\\
            1 & 1 & 1 & \ddots & \vdots\\
            0 & 1 & \ddots & \ddots  & 0\\
            \vdots & \ddots & \ddots & \ddots & 1\\
            0 & \dots & 0 & 1 & 1
        \end{vmatrix}
    \]
    \normalsize
    This is a tridiagonal matrix with ones on each diagonal. So this term is just
    $\abs{T_{n-1}}$.
\end{frame}


\begin{frame}
\frametitle{The Recursive Formula}
    \textbf{Second term}
    \small
    \[
        A_n=
        \left(\begin{array}{c>{\columncolor{red!20}}cccccc}
            \rowcolor{red!20}
            1 & 1 & 0 & 0 & \dots & 0 & 1\\
            1 & 1 & 1 & 0 & \dots & \dots & 0\\
            0 & 1 & \ddots & \ddots & \ddots & \ddots & \vdots\\
            0 & 0 & \ddots & \ddots & \ddots & \vdots & \vdots\\
            \vdots & \vdots & \ddots & \ddots & \ddots & \ddots & 0\\
            0 & \vdots & \dots & \ddots & \ddots & \ddots & 1\\
            1 & 0 & \dots & \dots & 0 & 1 & 1
        \end{array}\right)
        \hspace{.1in}
        (-1)^{1+2}
        \underbrace{
        \begin{vmatrix}
            1 & 1 & 0 & \dots & 0\\
            0 & 1 & 1 & \ddots & \vdots\\
            0 & 1 & \ddots & \ddots  & 0\\
            \vdots & \ddots & \ddots & \ddots & 1\\
            1 & \dots & 0 & 1 & 1
        \end{vmatrix}}_{\abs{B_{n-1}}}
    \]
    \normalsize
    We denote this matrix by $B_{n-1}$.
\end{frame}

\begin{frame}
\frametitle{The Recursive Formula}
    \textbf{Third term}
    \small
    \[
        A_n=
        \left(\begin{array}{cccccc>{\columncolor{red!20}}c}
            \rowcolor{red!20}
            1 & 1 & 0 & 0 & \dots & 0 & 1\\
            1 & 1 & 1 & 0 & \dots & \dots & 0\\
            0 & 1 & \ddots & \ddots & \ddots & \ddots & \vdots\\
            0 & 0 & \ddots & \ddots & \ddots & \vdots & \vdots\\
            \vdots & \vdots & \ddots & \ddots & \ddots & \ddots & 0\\
            0 & \vdots & \dots & \ddots & \ddots & \ddots & 1\\
            1 & 0 & \dots & \dots & 0 & 1 & 1
        \end{array}\right)
        \hspace{.1in}
        (-1)^{1+n}
        \underbrace{
        \begin{vmatrix}
            1 & 1 & 1 & \dots & 0\\
            0 & 1 & 1 & \ddots & \vdots\\
            0 & 0 & \ddots & \ddots  & 1\\
            \vdots & \ddots & \ddots & \ddots & 1\\
            1 & \dots & 0 & 0 & 1
        \end{vmatrix}}_{\abs{C_{n-1}}}
    \]
    \normalsize
    We denote this matrix by $C_{n-1}$.
\end{frame}

\begin{frame}
    \frametitle{The Recursive Formula}
    So far we have
    \[
        \abs{A_n} = \abs{T_{n-1}} - \abs{B_{n-1}} + (-1)^{n+1} \abs{C_{n-1}}
    \]
    We now perform cofactor expansion on $B_{n-1}$ and $C_{n-1}$ as well.
\end{frame}

\begin{frame}
\frametitle{The Recursive Formula}
    We expand on the first column of $B_{n-1}$, giving us two terms.
    \bigskip

    \textbf{First term}
    \small
    \[
        B_{n-1} = 
        \left(\begin{array}{>{\columncolor{red!20}}ccccccc}
            \rowcolor{red!20}
            1 & 1 & 0 & \dots & 0\\
            0 & 1 & 1 & \ddots & \vdots\\
            0 & 1 & \ddots & \ddots  & 0\\
            \vdots & \ddots & \ddots & \ddots & 1\\
            1 & \dots & 0 & 1 & 1
        \end{array}\right)
        \hspace{.1in}
        (-1)^{1+1}
        \begin{vmatrix}
            1 & 1 & 0 & \dots & 0\\
            1 & 1 & 1 & \ddots & \vdots\\
            0 & 1 & \ddots & \ddots & 0\\
            \vdots & \ddots & \ddots & \ddots & 1\\
            0 & \dots & 0 & 1 & 1
        \end{vmatrix}
    \]
    This is the tridiagonal matrix $T_{n-2}$.
    \normalsize
\end{frame}

\begin{frame}
\frametitle{The Recursive Formula}
    We expand on the first column of $B_{n-1}$, giving us two terms.
    \bigskip

    \textbf{Second term}
    \small
    \[
        B_{n-1} = 
        \left(\begin{array}{>{\columncolor{red!20}}ccccccc}
            1 & 1 & 0 & \dots & 0\\
            0 & 1 & 1 & \ddots & \vdots\\
            0 & 1 & \ddots & \ddots  & 0\\
            \vdots & \ddots & \ddots & \ddots & 1\\
            \rowcolor{red!20}
            1 & \dots & 0 & 1 & 1
        \end{array}\right)
        \hspace{.1in}
        (-1)^{n-1+1}
        \begin{vmatrix}
            1 & 0 & 0 & \dots & 0\\
            1 & 1 & 0 & \ddots & \vdots\\
            1 & \ddots & \ddots & \ddots & 0\\
            \vdots & \ddots & \ddots & \ddots & 0\\
            0 & \dots & 1 & 1 & 1
        \end{vmatrix}
    \]
    This is a lower triangular matrix with $1$s along the diagonal. So its determinant
    is $1$.
    \normalsize
\end{frame}

\begin{frame}
\frametitle{The Recursive Formula}

We have obtained the following formula for $\abs{B_{n-1}}$:
\[
    \abs{B_{n-1}} = \abs{T_{n-2}} + (-1)^n
\]
\end{frame}

\begin{frame}
\frametitle{The Recursive Formula}
    We expand on the first column of $C_{n-1}$, giving us two terms.
    \bigskip

    \textbf{First term}
    \small
    \[
        C_{n-1} = 
        \left(\begin{array}{>{\columncolor{red!20}}ccccccc}
            \rowcolor{red!20}
            1 & 1 & 1 & \dots & 0\\
            0 & 1 & 1 & \ddots & \vdots\\
            0 & 0 & \ddots & \ddots  & 1\\
            \vdots & \ddots & \ddots & \ddots & 1\\
            1 & \dots & 0 & 0 & 1
        \end{array}\right)
        \hspace{.1in}
        (-1)^{1+1}
        \begin{vmatrix}
            1 & 1 & 1 & \dots & 0\\
            0 & 1 & 1 & \ddots & \vdots\\
            0 & \ddots & \ddots & \ddots & 1\\
            \vdots & \ddots & \ddots & \ddots & 1\\
            0 & \dots & \dots & 0 & 1
        \end{vmatrix}
    \]
    This is an upper triangular matrix with $1$s along its diagonal. So its determinant
    is $1$.
    \normalsize
\end{frame}

\begin{frame}
\frametitle{The Recursive Formula}
    We expand on the first column of $C_{n-1}$, giving us two terms.
    \bigskip

    \textbf{Second term}
    \small
    \[
        C_{n-1} = 
        \left(\begin{array}{>{\columncolor{red!20}}ccccccc}
            1 & 1 & 1 & \dots & 0\\
            0 & 1 & 1 & \ddots & \vdots\\
            0 & 0 & \ddots & \ddots  & 1\\
            \vdots & \ddots & \ddots & \ddots & 1\\
            \rowcolor{red!20}
            1 & \dots & 0 & 0 & 1
        \end{array}\right)
        \hspace{.1in}
        (-1)^{n-1+1}
        \begin{vmatrix}
            1 & 1 & 0 & \dots & 0\\
            1 & 1 & 1 & \ddots & \vdots\\
            0 & 1 & \ddots & \ddots & 0\\
            \vdots & \ddots & \ddots & \ddots & 1\\
            0 & \dots & 0 & 1 & 1
        \end{vmatrix}
    \]
    This is the tridiagonal matrix $T_{n-2}$ again.
    \normalsize
\end{frame}

\begin{frame}
\frametitle{The Recursive Formula}

For $\abs{C_{n-1}}$ we have:
\[
    \abs{C_{n-1}} = 1 + (-1)^n\abs{T_{n-2}}
\]
\end{frame}

\begin{frame}
\frametitle{The Recursive Formula}

We substitute into the formula for $\abs{A_n}$:
\pause
    \begin{align*}
        \abs{A_n} &= \abs{T_{n-1}} - \abs{B_{n-1}} + (-1)^{n+1}\abs{C_{n-1}} \\
        &= \abs{T_{n-1}} - \left( \abs{T_{n-2}} + (-1)^n \right) + (-1)^{n+1}\left( 1 +
            (-1)^n \abs{T_{n-2}} \right)\\
        &= \abs{T_{n-1}} - \abs{T_{n-2}} + 2(-1)^{n+1} + (-1)^{2n+1}\abs{T_{n-2}}\\
        &= \abs{T_{n-1}} - 2\abs{T_{n-2}} + 2(-1)^{n+1}
    \end{align*}
    \pause
    But when is $\abs{A_n} = 0$? We claim if and only if $n \equiv 0 \pmod{3}$.
\end{frame}

\begin{frame}
\frametitle{The Recursive Formula}
Recall that $\abs{T_n}$ is given by 
\[
    \abs{T_n} = 
    \begin{cases}
        1 & n \equiv 0, 1 \pmod{6},\\
        0 & n \equiv 2, 5 \pmod{6},\\
        -1 & n \equiv 3,4 \pmod{6}.
    \end{cases}
\]
\end{frame}

\begin{frame}
\frametitle{The Recursive Formula}

$(\Rightarrow):$ If $\abs{A_n}=0$, then
\[
    \abs{A_n} = \abs{T_{n-1}} - 2\abs{T_{n-2}} + 2(-1)^{n+1} = 0
\]
\pause
But $\abs{T_{n-1}}$ and $\abs{T_{n-2}}$ only take on the values $0$,$1$, $-1$ so\ldots
\[
    \abs{A_n} = \{1,-1,0\} + \{2,-2,0\} + \{2,-2\} = 0
\]
\pause
So we must have that $\abs{T_{n-1}} = 0$. 
\pause

But then $n\equiv 0,3 \pmod{6}$ i.e. $n\equiv 0 \pmod{3}$.
\end{frame}

\begin{frame}
\frametitle{The Recursive Formula}

$(\Leftarrow):$ If $n\equiv 0 \pmod 3$ we have two possibilities for $n$ mod $6$:
\pause
\begin{enumerate}
    \item $n\equiv 0 \pmod{6}$, so $\abs{T_{n-1}} = 0$, $\abs{T_{n-2}}=-1$ and $n$ is
        even.
        \[ 
            \abs{A_n} = \abs{T_{n-1}} - 2\abs{T_{n-2}} + 2(-1)^{n+1} = 0 + 2 -2 = 0.
        \]
        \pause
    \item $n\equiv 3 \pmod{6}$, so $\abs{T_{n-1}} = 0$, $\abs{T_{n-2}}=1$ and $n$ is
        odd.
        \[ 
            \abs{A_n} = \abs{T_{n-1}} - 2\abs{T_{n-2}} + 2(-1)^{n+1} = 0 - 2 +2 = 0.
        \]
\end{enumerate}
\end{frame}


\end{document}


